$$
\lim_{x \to 0}{\frac{\ln(x+1)}{x}}
= \lim_{x\to 0}{e^{\ln{\frac{\ln(x+1)}{x}}}}
$$
$$
\lim_{x \to 0}{e^{\ln(x+1) - \ln(x)}} = {e^{\ln(1)-\ln(0)}} = {e^{\infty}}
$$
$$
\lim_{n \to \infty}{\sqrt[n]{\frac{2^n+3^n}{n^2+n^3}}} = \sqrt[n]{\frac{3^n(\frac{2^n}{3^n}+1)}{n^3(\frac{1}{n}+1)}} = \frac{3}{\sqrt[n]{n^3}}(\sqrt[n]{\frac{\frac{2^n}{3^n}+1}{\frac{1}{n}+1}}) = 3 (1) = 3
$$
$$
\lim_{n \to \infty}{\sqrt[n]{(n+1)^n-n^n}}
$$
$$
\lim_{n \to \infty}{\sqrt[n]{\sum_{k=0}^{n}\binom{n}{k}n^{n-k}1^{k}-n^n}}
$$
$$
\lim_{n \to \infty}{\sqrt[n]{n^n + \sum_{k=0}^{n-1}\binom{n}{k}n^{n-k}1^{k}-n^n}}
$$
$$
\lim_{n \to \infty}{\sqrt[n]{\sum_{k=0}^{n-1}\binom{n}{k}n^{n-k}1^{k}}} = \infty
$$
ex 4.7 (4) Apostol
$$
\sum_{k=1}^{n}{2k-1} = 2\sum_{k=1}^{n}{k-\frac{1}{2}} =  2(\sum_{k=1}^{n}{k}-\sum_{k=1}^{n}{\frac{1}{2}}) = 2(\sum_{k=1}^{n}{k} - \frac{n}{2}) = 2\sum_{k=1}^{n}{k} -n = 2(\frac{n(n+1)}{2}) -n = n^2 +n -n = n^2
$$